A12Kernel/Proofs.lean
@@ -197,6 +197,7 @@ import A12Kernel.Proofs.BooleanFirstFilledComputation
 import A12Kernel.Proofs.AddressedBooleanFirstFilledComputation
 import A12Kernel.Proofs.ExactTokenComputationResult
 import A12Kernel.Proofs.CustomFirstFilledComputation
+import A12Kernel.Proofs.AddressedCustomFirstFilledComputation
 import A12Kernel.Proofs.DateFragmentFirstFilledComputation
 import A12Kernel.Proofs.DateRangeFirstFilledComputation
 import A12Kernel.Proofs.DateTimeFirstFilledComputation
